theories/iris/language/lwp_resources.v
@@ -13,39 +13,44 @@ Section lwp_resources.
   Lemma lenient_wp_get_local s E (v: value) i Φ f :
     (f_locs f) !! i = Some v ->
     ▷Φ.(lp_val) [v] ∗
-    ▷Φ.(lp_fr) f ∗
+    Φ.(lp_fr) f ∗
+    Φ.(lp_fr_inv) f ∗
     ↪[frame] f ∗
     ↪[RUN]
     ⊢ lenient_wp s E [AI_basic (BI_get_local i)] Φ.
   Proof.
-    iIntros "%Hi (Hval & Hfr & Hf & Hrun)".
+    iIntros "%Hi (Hval & Hfr & Hfrinv & Hf & Hrun)".
     unfold lenient_wp.
     iApply (wp_wand with "[Hfr Hf Hrun Hval]").
     iApply (wp_get_local with "[Hfr Hval] [$] [$]").
     - by apply Hi.
-    - instantiate (1:=(fun v: iris.val => (lp_noframe Φ v ∗ lp_fr Φ f)%I)).
-      iFrame.
+    - instantiate (1:= (λ v, ↪[RUN] -∗ lp_noframe Φ f v)).
+      iIntros "!> ?"; iFrame.
     - iIntros (v0) "[[Hq Hrun] Hf]".
       unfold denote_logpred.
       iFrame.
+      by iApply "Hq".
   Qed.
 
   Lemma lenient_wp_set_local s E i Φ v (f: datatypes.frame) :
+    let f' := {| f_locs := seq.set_nth v (f_locs f) i v; f_inst := f_inst f |} in
     i < length f.(f_locs) ->
     ▷ Φ.(lp_val) [] ∗
+    ▷ Φ.(lp_fr) f' ∗
+    Φ.(lp_fr_inv) f' ∗
     ↪[frame] f ∗
     ↪[RUN]
-    ⊢ lenient_wp s E [AI_basic (BI_const v); AI_basic (BI_set_local i)] (lp_run (lp_fr_set f i v Φ)).
+    ⊢ lenient_wp s E [AI_basic (BI_const v); AI_basic (BI_set_local i)] Φ.
   Proof.
-    iIntros (Hlen) "(Hval & Hf & Hrun)".
-    iApply (wp_wand with "[Hval Hf Hrun]").
-    iApply (wp_set_local with "[Hval] [$Hf] [$Hrun]").
+    iIntros (f' Hlen) "(Hval & Hfr & Hfrinv & Hf & Hrun)".
+    iApply (wp_wand with "[Hval Hf Hfr Hrun]").
+    iApply (wp_set_local with "[Hval Hfr] [$Hf] [$Hrun]").
     - assumption.
-    - instantiate (1:= lp_noframe (lp_fr_set f i v Φ)).
-      by cbn.
+    - instantiate (1:= (λ v, ↪[RUN] -∗ lp_noframe Φ f' v)).
+      iIntros "!> ?"; iFrame.
     - iIntros (w) "((Hpred & Hrun) & Hf)".
-      iApply lp_with_sep.
-      by iFrame.
+      iSpecialize ("Hpred" with "Hrun").
+      iFrame.
   Qed.
 
   Theorem lenient_wp_tee_local s E i Φ v (f: datatypes.frame) :
@@ -65,46 +70,55 @@ Section lwp_resources.
     let R := N.of_nat n ↦[wms][Wasm_int.N_of_uint i32m k + off] bits v in
     is_true (types_agree t v) ->
     inst_memory (f_inst f) !! i = Some n ->
-    R ∗
     ↪[RUN] ∗
-    ▷ Φ.(lp_val) [v] ∗
+    R ∗
+    ▷ (R -∗ Φ.(lp_val) [v]) ∗
     Φ.(lp_fr) f ∗
+    Φ.(lp_fr_inv) f ∗
     ↪[frame] f
     ⊢ lenient_wp s E [AI_basic (BI_const (VAL_int32 k)); AI_basic (BI_load i t None a off)]
-                     (lp_with (R ∗ ↪[RUN]) Φ).
+                     Φ.
   Proof.
-    iIntros (R Hag Hmem) "(Hwp & Hrun & Hval & Hfr & Hf)".
-    iApply (wp_wand with "[Hwp Hrun Hval Hfr Hf]").
+    iIntros (R Hag Hmem) "(Hrun & HR & Hval & Hfr & Hfrinv & Hf)".
+    iApply (wp_wand with "[Hrun HR Hval Hfr Hf]").
     iApply wp_load; eauto.
     - iFrame.
-      instantiate (1:=(fun v: iris.val => (lp_noframe Φ v ∗ lp_fr Φ f)%I)).
+      instantiate (1:= (λ v, ↪[RUN] -∗ R -∗ lp_noframe Φ f v)).
+      cbn.
+      iIntros "!> ?"; iFrame.
+    - iIntros (v0) "[(Hnoframe & HR & Hrun) Hf]".
+      iSpecialize ("Hnoframe" with "Hrun").
       iFrame.
-    - iIntros (v0) "[[[Hnoframe Hfr] [HR Hrun]] Hf]".
-      rewrite -lp_with_sep.
-      iFrame.
+      by iApply "Hnoframe".
   Qed.
 
   Theorem lenient_wp_store Φ s E t bs v off a k n f i :
+    let R := N.of_nat n↦[wms][Wasm_int.N_of_uint i32m k + off] bs in
+    let R' := N.of_nat n↦[wms][Wasm_int.N_of_uint i32m k + off]bits v in
     is_true (types_agree t v) ->
     length bs = length_t t ->
     inst_memory (f_inst f) !! i = Some n ->
-    N.of_nat n↦[wms][Wasm_int.N_of_uint i32m k + off] bs ∗
+    R ∗
     ↪[RUN] ∗
-    ▷ Φ.(lp_val) [] ∗
+    ▷ (R' -∗ Φ.(lp_val) []) ∗
     Φ.(lp_fr) f ∗
+    Φ.(lp_fr_inv) f ∗
     ↪[frame] f
-    ⊢ lenient_wp s E [AI_basic (BI_const (VAL_int32 k)); AI_basic (BI_const v); AI_basic (BI_store i t None a off)]
-                     (lp_with (N.of_nat n↦[wms][Wasm_int.N_of_uint i32m k + off]bits v ∗ ↪[RUN]) Φ).
+    ⊢ lenient_wp s E [AI_basic (BI_const (VAL_int32 k));
+                      AI_basic (BI_const v);
+                      AI_basic (BI_store i t None a off)]
+                     Φ.
   Proof.
-    iIntros (Hag Hlen Hmem) "(Hptr & Hrun & Hval & Hfr & Hf)".
-    iApply (wp_wand with "[Hptr Hrun Hval Hf]").
-    - iFrame.
-      iApply wp_store; eauto.
-      instantiate (1:=(fun v: iris.val => lp_noframe Φ v)).
+    iIntros (R R' Hag Hlen Hmem) "(HR & Hrun & Hval & Hfr & Hfrinv & Hf)".
+    iApply (wp_wand with "[HR Hrun Hval Hf Hfr]").
+    - iApply wp_store; eauto.
       iFrame.
-    - iIntros (v0) "[[Hnofram [Hptr Hrun]] Hf]".
-      rewrite -lp_with_sep.
+      instantiate (1:= (λ v, ↪[RUN] -∗ R' -∗ lp_noframe Φ f v)).
+      cbn.
+      iIntros "!> ?"; iFrame.
+    - iIntros (v0) "[[Hnoframe [Hptr Hrun]] Hf]".
       iFrame.
+      iApply ("Hnoframe" with "[$] [$]").
   Qed.
 
 End lwp_resources.
